Prove one_step_unique

coq/untyped.v
@@ -7,22 +7,117 @@ Inductive term : Type :=
 | tmpred : term -> term
 | tmiszero : term -> term.
 
-Definition subterm (s : term) (t : term) : Prop :=
-  match t with
-  | tmtrue => False
-  | tmfalse => False
-  | tmif t1 t2 t3 => t1 = s \/ t2 = s \/ t3 = s
-  | tmzero => False
-  | tmsucc t' => t' = s
-  | tmpred t' => t' = s
-  | tmiszero t' => t' = s
-  end.
+Inductive is_numeric_val : term -> Prop :=
+| N_Zero :
+    is_numeric_val tmzero
+| N_Succ : forall t,
+    is_numeric_val t ->
+    is_numeric_val (tmsucc t).
 
-Theorem term_struct_ind : forall P : term -> Prop, (forall s : term, (forall r: term, subterm r s -> P r) -> P s) -> (forall t : term, P t).
-  intros P H.
-  induction t; apply H; intros r H'; simpl in H'; try contradiction.
-  -repeat (destruct H' as [H' | H']; try (rewrite <- H'; assumption)).
-  -repeat (rewrite <- H'; assumption).
-  -rewrite <- H'; assumption.
-  -rewrite <- H'; assumption.
+Inductive subterm : term -> term -> Prop :=
+| S_IfCond : forall t t1 t2,
+    subterm t (tmif t t1 t2)
+| S_IfTrue : forall t t1 t2,
+    subterm t1 (tmif t t1 t2)
+| S_IfFalse : forall t t1 t2,
+    subterm t2 (tmif t t1 t2)
+| S_Succ : forall t,
+    subterm t (tmsucc t)
+| S_Pred : forall t,
+    subterm t (tmpred t)
+| S_IsZero : forall t,
+    subterm t (tmiszero t).
+
+Reserved Notation "x --> y" (at level 80, no associativity).
+
+Inductive one_step : term -> term -> Prop :=
+| E_IfTrue : forall t t',
+    (tmif tmtrue t t') --> t
+| E_IfFalse : forall t t',
+    (tmif tmfalse t t') --> t'
+| E_If : forall t t' t1 t2,
+    (t --> t') ->
+    ((tmif t t1 t2) --> (tmif t' t1 t2))
+| E_Succ : forall t t',
+    (t --> t') ->
+    tmsucc t --> tmsucc t'
+| E_PredZero :
+    tmpred tmzero --> tmzero
+| E_PredSucc : forall nv,
+    is_numeric_val nv ->
+    tmpred (tmsucc nv) --> nv
+| E_IsZeroZero :
+    tmiszero tmzero --> tmtrue
+| E_IsZeroSucc : forall nv,
+    is_numeric_val nv ->
+    tmiszero (tmsucc nv) --> tmfalse
+| E_IsZero : forall t t',
+    t --> t' ->
+    tmiszero t --> tmiszero t'
+
+where "x --> y" := (one_step x y).
+
+Lemma numericval_no_eval : forall nv, is_numeric_val nv -> (forall t, not (nv --> t)).
+  intros nv H.
+  induction H; unfold not. intros.
+  -inversion H.
+  -intros t' H'.
+   inversion H'; subst.
+   specialize (IHis_numeric_val t'0).
+   apply IHis_numeric_val.
+   assumption.
+Qed.
+   
+Lemma one_step_unique : forall t t1 t2, t --> t1 -> t --> t2 -> t1 = t2.
+  intros t t1 t2 H1 H2.
+  generalize dependent t2.
+  induction H1.
+  -intros t2 H2. (* E_IfTrue *)
+   inversion H2.
+   +reflexivity.
+   +inversion H4.
+  -intros t2 H2. (* E_IfFalse *)
+   inversion H2; subst.
+   +reflexivity.
+   +inversion H4.
+  -intros t0 H0. (* E_If *)
+   inversion H0; subst.
+   +inversion H1.
+   +inversion H1.
+   +specialize (IHone_step t'0).
+    specialize (IHone_step H5).
+    rewrite IHone_step.
+    reflexivity.
+  -intros t2 H. (* E_Succ *)
+   inversion H; subst.
+   specialize (IHone_step t'0).
+   rewrite (IHone_step H2); reflexivity.
+  -intros. (* E_PredZero *)
+   inversion H2; reflexivity.
+  -intros. (* E_PredSucc *)
+   inversion H2; subst; reflexivity.
+  -intros. (* E_IsZeroZero *)
+   inversion H2; subst.
+   +reflexivity.
+   +inversion H0.
+  -intros. (* E_IsZeroSucc *)
+   inversion H2; subst.
+   +reflexivity.
+   +inversion H1; subst.
+    apply numericval_no_eval in H3.
+    contradiction.
+    apply numericval_no_eval in H3.
+    assumption.
+    apply numericval_no_eval in H3.
+    contradiction.
+    apply H.
+  -intros t2 H. (* E_IsZero *)
+   inversion H; subst.
+   +inversion H1.
+   +apply numericval_no_eval in H1.
+    contradiction.
+    apply N_Succ; assumption.
+   +specialize (IHone_step t'0).
+    rewrite (IHone_step H2).
+    reflexivity.
 Qed.
